Denotational-Common.thy
@@ -33,7 +33,7 @@ instance
   done
 end
 
-lemma sharp_star_Env: "set (bn as) \<sharp>* (\<rho> :: Env) \<longleftrightarrow> (\<forall> x \<in> fst`set (asToHeap as) . x \<notin> fdom \<rho>)"
+lemma sharp_star_Env: "set (bn as) \<sharp>* (\<rho> :: Env) \<longleftrightarrow> (\<forall> x \<in> heapVars (asToHeap as) . x \<notin> fdom \<rho>)"
   by(induct rule:asToHeap.induct, auto simp add: fresh_star_def exp_assn.bn_defs sharp_Env)
 
 end
